Tweaks, fixes, and dead code removal

theories/language/wp_link.v
@@ -19,7 +19,7 @@ Implicit Types Ψ : protocol val Σ.
 Implicit Types prog : lang_prog Λ.
 Implicit Types pe : prog_environ Λ Σ.
 
-
+(*
 Definition program_fulfills
   (Ψin : protocol val Σ) (p : mixin_prog (func Λ)) (Ψshould : protocol val Σ) : iProp Σ :=
   ∀ s vv Φ, Ψshould s vv Φ -∗ ⌜p !! s <> None⌝ ∗ WP (of_class _ (ExprCall s vv)) @ ⟨p, Ψin⟩; ⊤ {{ Φ }}.
@@ -33,14 +33,14 @@ Definition spec_union (p1 p2 : protocol val Σ) : protocol val Σ :=
   λ s vv Φ, (p1 s vv Φ ∨ p2 s vv Φ)%I.
 Definition spec_inters (p1 p2 : protocol val Σ) : protocol val Σ :=
   λ s vv Φ, (p1 s vv Φ ∧ p2 s vv Φ)%I.
+*)
 
-
-Class can_link (Ψ1 Ψ2 Ψaxiom Ψres : protocol val Σ) (p1 p2 p3 : lang_prog Λ) : Prop := {
+Class can_link E (Ψ1 Ψ2 Ψaxiom Ψres : protocol val Σ) (p1 p2 p3 : lang_prog Λ) : Prop := {
   p1_p2_disjoint : dom p1 ## dom p2;
-  Ψres_is_union : ⊢ (∀ s vv Φ, Ψres s vv Φ -∗ (spec_union Ψ1 Ψ2) s vv Φ)%I;
+  Ψres_is_union : ⊢ (∀ s vv Φ, Ψres s vv Φ -∗ (Ψ1 ⊔ Ψ2) s vv Φ)%I;
   Ψaxiom_is_axiomatic : ⊢ (∀ s vv Φ, Ψaxiom s vv Φ -∗ ⌜s ∉ dom p3⌝)%I;
-  p1_satisfies_Ψ1 : ⊢ (spec_union Ψ2 Ψaxiom |- p1 :: Ψ1)%I;
-  p2_satisfies_Ψ2 : ⊢ (spec_union Ψ1 Ψaxiom |- p2 :: Ψ2)%I;
+  p1_satisfies_Ψ1 : (Ψ2 ⊔ Ψaxiom ||- p1 @ E :: Ψ1);
+  p2_satisfies_Ψ2 : (Ψ1 ⊔ Ψaxiom ||- p2 @ E :: Ψ2);
   p3_is_union : p3 = (union_with (λ _ _ : func Λ, None) p1 p2);
 }.
 
@@ -108,21 +108,21 @@ Proof.
   exists p. split; eauto. by apply elem_of_list_In.
 Qed.
 
-Class can_link_all 
+Class can_link_all E
     (Ψaxiom Ψres : protocol val Σ) (pres : lang_prog Λ)
     (A : list (prod (protocol val Σ) (lang_prog Λ))) := {
   all_disjoint : pairwise (map snd A) (fun p1 p2 => dom p1 ## dom p2);
   Ψres_is_big_union : ⊢ (∀ s vv Φ, Ψres s vv Φ -∗ (spec_union_list (map fst A)) s vv Φ)%I;
   Ψaxiom_is_axiomatic_all : ⊢ (∀ s vv Φ, Ψaxiom s vv Φ -∗ ⌜s ∉ dom pres⌝)%I;
   pres_is_union : pres = union_map_list (map snd A);
-  one_spec := fun i => spec_union (spec_union_list_except i (map fst A)) Ψaxiom;
+  one_spec := fun i => (spec_union_list_except i (map fst A)) ⊔ Ψaxiom;
   all_satisfy_spec : ∀ i, match (nth_error A i) with None => True |
-      Some (Ψi, pi) =>  ⊢ (one_spec i |- pi :: Ψi)%I end
+      Some (Ψi, pi) =>  (one_spec i ||- pi @ E :: Ψi)%I end
 }.
 
 #[global]
-Instance can_link_can_link_all Ψaxiom Ψres pres Ψ1 Ψ2 p1 p2 : can_link Ψ1 Ψ2 Ψaxiom Ψres p1 p2 pres
-  -> can_link_all Ψaxiom Ψres pres [(Ψ1,p1); (Ψ2,p2)].
+Instance can_link_can_link_all E Ψaxiom Ψres pres Ψ1 Ψ2 p1 p2 : can_link E Ψ1 Ψ2 Ψaxiom Ψres p1 p2 pres
+  -> can_link_all E Ψaxiom Ψres pres [(Ψ1,p1); (Ψ2,p2)].
 Proof.
   intros [H1 H2 H3 H4 H5 H6]; split; cbn.
   - intros [|[|[|i]]] [|[|[|j]]] H; cbn; easy.
@@ -135,129 +135,116 @@ Proof.
     destruct (p1 !! i), (p2 !! i); done.
   - intros [|[|[|i]]]; cbn; try done.
     all: iIntros (s vv Φ) "Hres"; cbn.
-    1: iPoseProof H4 as "H"; iSpecialize ("H" $! s vv Φ with "Hres").
-    2: iPoseProof H5 as "H"; iSpecialize ("H" $! s vv Φ with "Hres").
-    all: iDestruct "H" as "[$ HWP]".
-    all: iApply wp_proto_mono; last iApply "HWP".
+    1: iPoseProof H4 as "H"; iSpecialize ("H" with "Hres").
+    2: iPoseProof H5 as "H"; iSpecialize ("H" with "Hres").
+    all: iDestruct "H" as "(%F&%HF&%e&%He&H)".
+    all: iExists F; iSplit; first done.
+    all: iExists e; iSplit; first done.
+    all: iNext.
+    all: iApply wp_proto_mono; last iApply "H".
     all: cbn; intros s' vv' Φ'; iIntros "[H|H]".
     2,4: by iRight. all: iLeft.
     1: iExists 1. 2: iExists 0.
     all: iSplitR; first done. all: done.
 Qed.
 
-Lemma wp_link_execs Ψaxiom Ψres (pres : gmap string (Λ.(func))) A :
-  can_link_all Ψaxiom Ψres pres A
+Lemma wp_link_execs E Ψaxiom Ψres (pres : gmap string (Λ.(func))) A :
+  can_link_all E Ψaxiom Ψres pres A
   -> ⊢ ∀ e Φ i, match (nth_error A i) with None => ⌜False⌝ | 
-          Some (Ψi, pi) => WP e @ ⟨pi, spec_union (spec_union_list_except i (map fst A)) Ψaxiom ⟩; ⊤ {{ Φ }} end
-     -∗ WP e @ ⟨pres, Ψaxiom⟩; ⊤ {{ Φ }}.
+          Some (Ψi, pi) => WP e @ ⟨pi, (spec_union_list_except i (map fst A)) ⊔ Ψaxiom ⟩; E {{ Φ }} end
+     -∗ WP e @ ⟨pres, Ψaxiom⟩; E {{ Φ }}.
 Proof.
   intros [Hdis HΨres Haxiom -> one_spec' Hsatis].
   iLöb as "IHe". iIntros (e Φ i).
   destruct (nth_error A i) as [[Ψi pi]|] eqn:Heq; last (iIntros "%H"; done).
   rewrite !wp_unfold /wp_pre /=.
   iIntros "H %σ Hσ".
-  - iSpecialize ("H" $! σ with "Hσ").
-    iMod "H".
-    iDestruct "H" as "[(%x & -> & Hσ & H)|[(%s' & %vv' & %K & %HeqK & %H2 & >(%Ξ & Hσ & [HΨ|HΨ] & H3))|(%HH & H3)]]".
-    * iModIntro. iLeft. iExists _. iFrame. iPureIntro. done.
-    * iDestruct "HΨ" as "(%kidx & %Hknei & HΨ)". rewrite nth_error_map.
-      destruct (nth_error A kidx) as [[Ψc pc]|] eqn:Heqk; cbn; last iPure "HΨ" as [].
-      specialize (Hsatis kidx). rewrite Heqk in Hsatis.
-      iPoseProof (Hsatis) as "Hsatis".
-      iDestruct ("Hsatis" $! s' vv' Ξ with "HΨ")as "(%HNone & HΨ)".
-      rewrite wp_unfold /wp_pre /=.
-      iSpecialize ("HΨ" $! σ with "Hσ").
-      iMod "HΨ" as "[(%x & %Heqx & Hσ & H)|[(%s'2 & %vv'2 & %K'2 & %HeqK2 & %H''2 & >(%Ξ' & Hσ & HΨ' & H3'))|(%HH2&H3')]]".
-      -- exfalso. apply of_class_inj in Heqx. congruence.
-      -- exfalso. assert (K'2 = empty_ectx) as ->. 
-         2: { rewrite fill_empty in HeqK2. apply of_class_inj in HeqK2. assert (s'2 = s') as -> by congruence; congruence. }
-         destruct (fill_class K'2 (of_class Λ (ExprCall s'2 vv'2))) as [H1|[x Hx]].
-         { eexists. rewrite <- HeqK2. by rewrite to_of_class. }
-        { done. }
-          { exfalso. unfold to_val in Hx. rewrite to_of_class in Hx; congruence. }
-     -- destruct HH2 as (e' & σ' & (KK & e1' & e2' & Heq2 & -> & Hstep)%prim_step_inv).
-          destruct (fill_class KK e1') as [->|[x Hx]].
-         { eexists. rewrite <- Heq2. by rewrite to_of_class. }
-         2: { apply val_head_stuck in Hstep. congruence. }
-         rewrite ! fill_empty in Heq2. subst e1'.
-         apply call_head_step in Hstep.
-         destruct Hstep as (Fn & Heqp2' & He2' & -> ). iRight. iRight.
-         assert (union_map_list (map snd A) !! s' = Some Fn) as Heqs'.
-         { apply union_map_list_spec; first done. exists pc; repeat split; try done.
-           apply in_map_iff. exists ((Ψc,pc)); repeat split. by eapply nth_error_In. }
-         iModIntro. iSplit; first iPureIntro.
-         { do 2 eexists. rewrite HeqK. econstructor; first done. 1:done.
-           apply call_head_step. exists Fn. repeat split; try done. }
-         subst e. iIntros (? ? (e'2 & -> & (Fn3 & Heqp3' & He3' & ->)%call_head_step)%head_reducible_prim_step_ctx).
-         2: { do 2 eexists.
-              apply call_head_step. exists Fn. repeat split; try done. }
-         rewrite Heqs' in Heqp3'. assert (e'2 = e2') as -> by congruence.
-         iSpecialize ("H3'" $! σ e2').
-         assert (prim_step pc (of_class Λ (ExprCall s' vv')) σ e2' σ) as Hstep2.
-         { apply head_prim_step. apply call_head_step. eexists; repeat split; done. }
-         iSpecialize ("H3'" $! Hstep2). iMod "H3'". iModIntro. iNext.
-         iMod "H3'" as "(? & H3')". iModIntro. iFrame.
-         iApply wp_bind. iApply (wp_wand with "[H3']").
-         { iApply ("IHe" $! _ _ kidx). rewrite Heqk. iApply "H3'". }
-         iIntros (r) "Hr". iSpecialize ("H3" $! r with "Hr"). iApply ("IHe" $! _ _ i). rewrite Heq. done.
-    * iRight. iLeft. iModIntro. do 3 iExists _; iSplitR; first done.
-      destruct (union_map_list (map snd A) !! s') as [v|] eqn:Heqv.
-      { iExFalso. iDestruct (Haxiom $! s' vv' Ξ with "HΨ") as "%Hfalse". exfalso.
-        apply Hfalse. eapply elem_of_dom_2. done. }
-      cbn. iSplitR; first done. iModIntro. iExists Ξ. iFrame. iNext.
-      iIntros (r) "Hr". iSpecialize ("H3" with "Hr"). iApply ("IHe" $! _ _ i). by rewrite Heq.
-    * iModIntro. iRight. iRight.
-      iSplitR.
-      { iPureIntro. eapply reducible_mono; last done.
-        apply union_map_subset; first done. apply elem_of_list_In.
-        apply in_map_iff. exists ((Ψi, pi)); split; eauto.
-        by eapply nth_error_In. }
-      iIntros (σ' e' Hstep%prim_step_inv).
-      iSpecialize ("H3" $! σ' e').
-      destruct Hstep as (K & e1' & e2' & -> & -> & H).
-      assert (prim_step pi (fill K e1') σ (fill K e2') σ') as Hstep.
-      { econstructor. 1-2:done. destruct (to_class e1') as [[]|] eqn:Heqe1.
-        - exfalso. eapply val_head_step. apply of_to_class in Heqe1. erewrite Heqe1. done.
-        - apply of_to_class in Heqe1. subst e1'.
-          destruct HH as (? & σ'2 & (e2'' & -> & (K2 & eK1 & eK2 & Heq1 & -> & HHstep)%prim_step_inv)%fill_step_inv).
-          2: unfold to_val; by rewrite to_of_class.
-          assert (K2 = empty_ectx) as ->.
-          1: { destruct (fill_class' K2 eK1) as [|[vv Hvv]].
-               1: eexists; rewrite <- Heq1; by rewrite to_of_class.
-               1: done.
-               exfalso. apply of_to_class in Hvv. subst eK1. eapply val_head_step. done. }
-          rewrite fill_empty in Heq1. subst eK1. apply call_head_step in H, HHstep.
-          destruct H as (FN1 & HFN1 &Happy1 & ->).
-          destruct HHstep as (FN2 & HFN2 &Happy2 & ->).
-          apply union_map_list_spec in HFN1; last done. destruct HFN1 as (? & [[ΨΨ kk] [<- (kki & Hkki)%In_nth_error]]%in_map_iff & HFN1).
-          cbn in HFN1. destruct (decide (kki = i)) as [-> | Hcontr].
-          1: apply call_head_step; exists FN2; repeat split; try congruence.
-          exfalso. specialize (Hdis kki i Hcontr). rewrite ! nth_error_map in Hdis.
-          rewrite Hkki in Hdis. rewrite Heq in Hdis. cbn in Hdis. rewrite elem_of_disjoint in Hdis.
-          eapply Hdis; eapply elem_of_dom_2; done.
-        - by eapply head_step_no_call. }
-      iDestruct ("H3" $! Hstep) as ">H3". iModIntro. iNext.
-      iMod "H3" as "(Hσ & HWP)". iModIntro. iFrame. iApply ("IHe" $! _ _ i). rewrite Heq. done.
+  iSpecialize ("H" $! σ with "Hσ").
+  iMod "H".
+  iDestruct "H" as "[(%x & -> & Hσ & H)|[(%s' & %vv' & %K & %HeqK & %H2 & >(%Ξ & Hσ & [HΨ|HΨ] & H3))|(%HH & H3)]]".
+  - iModIntro. iLeft. iExists _. iFrame. iPureIntro. done.
+  - iDestruct "HΨ" as "(%kidx & %Hknei & HΨ)". rewrite nth_error_map.
+    destruct (nth_error A kidx) as [[Ψc pc]|] eqn:Heqk; cbn; last iPure "HΨ" as [].
+    specialize (Hsatis kidx). rewrite Heqk in Hsatis.
+    iPoseProof (Hsatis) as "Hsatis".
+    iDestruct ("Hsatis" with "HΨ") as "(%F&%HF&%e'&%He'&HΨ)".
+    iRight. iRight. iModIntro.
+    assert (union_map_list (map snd A) !! s' = Some F) as HHF.
+    { apply union_map_list_spec. 1: apply Hdis.
+      exists pc. split; last done.
+      eapply nth_error_In, (in_map snd) in Heqk. apply Heqk. }
+    subst e. assert (head_reducible (union_map_list (map snd A)) ((of_class Λ (ExprCall s' vv'))) σ) as Hredu.
+    { do 2 eexists. eapply call_head_step. eexists. split_and!. 2: symmetry; apply He'. all:done. }
+    iSplit. 1: iPureIntro; eapply fill_reducible, head_prim_reducible, Hredu.
+    iIntros (σ' e'1 (e'2&->&(F2&HF2&He2&->)%call_head_step_inv)%head_reducible_prim_step_ctx); last done.
+    simplify_eq. assert (e'2 = e') as -> by congruence.
+    do 3 iModIntro. iFrame "Hσ".
+    iApply (wp_bind).
+    iApply ("IHe" $! _ _ kidx).
+    rewrite Heqk.
+    iApply (wp_wand with "HΨ").
+    iIntros (v) "Hv".
+    iApply ("IHe" $! _ _ i).
+    rewrite Heq.
+    iApply ("H3" with "Hv").
+  - iRight. iLeft. iModIntro. do 3 iExists _; iSplitR; first done.
+    destruct (union_map_list (map snd A) !! s') as [v|] eqn:Heqv.
+    { iExFalso. iDestruct (Haxiom $! s' vv' Ξ with "HΨ") as "%Hfalse". exfalso.
+      apply Hfalse. eapply elem_of_dom_2. done. }
+    cbn. iSplitR; first done. iModIntro. iExists Ξ. iFrame. iNext.
+    iIntros (r) "Hr". iSpecialize ("H3" with "Hr"). iApply ("IHe" $! _ _ i). by rewrite Heq.
+  - iModIntro. iRight. iRight.
+    iSplitR.
+    { iPureIntro. eapply reducible_mono; last done.
+      apply union_map_subset; first done. apply elem_of_list_In.
+      apply in_map_iff. exists ((Ψi, pi)); split; eauto.
+      by eapply nth_error_In. }
+    iIntros (σ' e' Hstep%prim_step_inv).
+    iSpecialize ("H3" $! σ' e').
+    destruct Hstep as (K & e1' & e2' & -> & -> & H).
+    assert (prim_step pi (fill K e1') σ (fill K e2') σ') as Hstep.
+    { econstructor. 1-2:done. destruct (to_class e1') as [[]|] eqn:Heqe1.
+      - exfalso. eapply val_head_step. apply of_to_class in Heqe1. erewrite Heqe1. done.
+      - apply of_to_class in Heqe1. subst e1'.
+        destruct HH as (? & σ'2 & (e2'' & -> & (K2 & eK1 & eK2 & Heq1 & -> & HHstep)%prim_step_inv)%fill_step_inv).
+        2: unfold to_val; by rewrite to_of_class.
+        assert (K2 = empty_ectx) as ->.
+        1: { destruct (fill_class' K2 eK1) as [|[vv Hvv]].
+             1: eexists; rewrite <- Heq1; by rewrite to_of_class.
+             1: done.
+             exfalso. apply of_to_class in Hvv. subst eK1. eapply val_head_step. done. }
+        rewrite fill_empty in Heq1. subst eK1. apply call_head_step in H, HHstep.
+        destruct H as (FN1 & HFN1 &Happy1 & ->).
+        destruct HHstep as (FN2 & HFN2 &Happy2 & ->).
+        apply union_map_list_spec in HFN1; last done. destruct HFN1 as (? & [[ΨΨ kk] [<- (kki & Hkki)%In_nth_error]]%in_map_iff & HFN1).
+        cbn in HFN1. destruct (decide (kki = i)) as [-> | Hcontr].
+        1: apply call_head_step; exists FN2; repeat split; try congruence.
+        exfalso. specialize (Hdis kki i Hcontr). rewrite ! nth_error_map in Hdis.
+        rewrite Hkki in Hdis. rewrite Heq in Hdis. cbn in Hdis. rewrite elem_of_disjoint in Hdis.
+        eapply Hdis; eapply elem_of_dom_2; done.
+      - by eapply head_step_no_call. }
+    iDestruct ("H3" $! Hstep) as ">H3". iModIntro. iNext.
+    iMod "H3" as "(Hσ & HWP)". iModIntro. iFrame. iApply ("IHe" $! _ _ i). rewrite Heq. done.
 Qed.
 
-Lemma wp_link_progs Ψaxiom Ψres (pres : gmap string (Λ.(func))) A :
-  can_link_all Ψaxiom Ψres pres A
- -> ⊢ Ψaxiom |- pres :: Ψres.
+Lemma wp_link_progs E Ψaxiom Ψres (pres : gmap string (Λ.(func))) A :
+  can_link_all E Ψaxiom Ψres pres A
+ -> Ψaxiom ||- pres @ E :: Ψres.
 Proof.
   intros [Hdis HΨres Haxiom -> one_spec' Hsatis].
   iIntros (s vv Φ) "H". iPoseProof HΨres as "HΨres".
-    iDestruct ("HΨres" with "H") as "[%x Hx]".
-    erewrite nth_error_map.
-    destruct (nth_error A x) as [[Ψi pi]|] eqn:Heq; last by iExFalso. cbn.
-    specialize (Hsatis x) as Hsatis2.
-    rewrite Heq in Hsatis2. iDestruct (Hsatis2 $! s vv Φ with "Hx") as "[%Hx1 Hx2]".
-    destruct (union_map_list (map snd A) !! s) eqn:Hl2.
-  - iSplitR; first done. unshelve iApply (wp_link_execs _ _ _ _ $! _ _ x). 3: by split. rewrite Heq. done.
-  - exfalso. destruct (pi !! s) as [f|] eqn:Heqpi; try congruence.
-    assert (∃ k, In k ((map snd A)) ∧ k !! s = Some f) as HH.
-    + exists pi; repeat split; try done. apply in_map_iff. exists (Ψi,pi).
-      repeat split; try done. eapply nth_error_In. done.
-    + apply union_map_list_spec in HH; try congruence. done.
+  iDestruct ("HΨres" with "H") as "[%x Hx]".
+  erewrite nth_error_map.
+  destruct (nth_error A x) as [[Ψi pi]|] eqn:Heq; last by iExFalso. cbn.
+  specialize (Hsatis x) as Hsatis2.
+  rewrite Heq in Hsatis2. iDestruct (Hsatis2 with "Hx") as "(%F&%HF&%e&%He&H)".
+  iExists F. iSplit.
+  - iPureIntro. apply union_map_list_spec. 1: apply Hdis.
+    exists pi. split; last done.
+    eapply nth_error_In, (in_map snd) in Heq. apply Heq.
+  - iExists e. iSplit; first done. iNext.
+    iApply (wp_link_execs). 1: done.
+    erewrite Heq. iApply "H".
 Qed.
 
 
